.github/PULL_REQUEST_TEMPLATE.md
@@ -6,20 +6,3 @@
 
 
 By submitting this pull request, I confirm that my contribution is made under the terms of the Apache 2.0 license.
-
-# Due to [dafny-lang/dafny#2500](https://github.com/dafny-lang/dafny/issues/2500), Traits are dangerous:
-1. [ ] Does this PR add any traits or classes that extend a trait?
-2. [ ] Are these traits annotated with `{:termination false}`?
-
-The override checks on 
-the specifications on
-a class' functions/methods/etc. validating
-that specifications are 
-at least as strong as those on
-the traits it implements
-are not working correctly when 
-that trait is defined in a different module 
-(and hence must have `{:termination false}` on it).
-
-As such, if either (1.) or (2.) is true:
-- [ ] manually verified all the trait specifications are copied onto classes that extend them?
