ComAmazonawsKms/runtimes/java/build.gradle.kts
@@ -52,7 +52,7 @@ repositories {
 }
 
 dependencies {
-    implementation("dafny.lang:DafnyRuntime:3.10.0")
+    implementation("org.dafny:DafnyRuntime:4.0.0")
     implementation("software.amazon.dafny:conversion:1.0-SNAPSHOT")
     implementation("software.amazon.cryptography:StandardLibrary:1.0-SNAPSHOT")
     implementation(platform("software.amazon.awssdk:bom:2.19.1"))
